reachabiliby rework, observability experiments

FSM.thy
@@ -9,6 +9,56 @@ record ('in, 'out, 'state) FSM =
   outputs :: "'out set"
   transitions :: "('state * 'in * 'out * 'state) set"
 
+
+
+(*
+inductive enabled_transition_seq :: "('in, 'out, 'state) FSM \<Rightarrow> 'state \<Rightarrow> (('in * 'out) * 'state) list => bool" where
+ets_nil  : "enabled_transition_seq M s Nil" |
+ets_one  : "(s1,x,y,s2) \<in> transitions M \<Longrightarrow> enabled_transition_seq M s1 (((x,y),s2)#Nil)" |
+ets_long : "(s1,x,y,s2) \<in> transitions M \<Longrightarrow> enabled_transition_seq M s2 seq \<Longrightarrow> enabled_transition_seq M s1 (((x,y),s2)#seq)"
+
+inductive reachable :: "('in, 'out, 'state) FSM \<Rightarrow> 'state \<Rightarrow> bool" where
+reachable_init : "reachable M (initial M)" |
+reachable_immediately : "((initial M),x,y,s2) \<in> transitions M \<Longrightarrow> reachable M s2" |
+reachable_distant : "(s2,x,y,s3) \<in> transitions M \<Longrightarrow> reachable M s2 \<Longrightarrow> reachable M s3"
+
+inductive reaches :: "('in, 'out, 'state) FSM \<Rightarrow> ('in * 'out) list \<Rightarrow> 'state \<Rightarrow> bool" where
+reaches_nil : "reaches M Nil (initial M)" |
+reaches_transition : "reaches M seq s1 \<Longrightarrow> (s1,x,y,s2) \<in> transitions M \<Longrightarrow> reaches M (seq@((x,y)#Nil)) s2"
+*)
+
+fun is_enabled_sequence :: "('in, 'out, 'state) FSM \<Rightarrow> 'state \<Rightarrow> ('state * 'in * 'out * 'state) list => bool" where
+"is_enabled_sequence M s Nil = True" |
+"is_enabled_sequence M s ((s1,x,y,s2)#seq) = (s = s1 \<and> (s1,x,y,s2) \<in> transitions M \<and> is_enabled_sequence M s2 seq)"
+
+print_theorems
+
+fun enabled_sequences :: "('in, 'out, 'state) FSM \<Rightarrow> 'state \<Rightarrow> ('state * 'in * 'out * 'state) list set" where
+"enabled_sequences M s = {seq . is_enabled_sequence M s seq}"
+
+fun get_io :: "('state * 'in * 'out * 'state) list \<Rightarrow> ('in * 'out) list" where
+"get_io seq = map (\<lambda> (s1,x,y,s2) . (x,y)) seq"
+
+definition is_enabled_io_sequence :: "('in, 'out, 'state) FSM \<Rightarrow> 'state \<Rightarrow> ('in * 'out) list => bool" where
+"is_enabled_io_sequence M s io \<equiv> \<exists> seq . is_enabled_sequence M s seq \<and> io = get_io seq"
+
+fun is_target :: "('state * 'in * 'out * 'state) list => 'state \<Rightarrow> bool" where
+"is_target Nil q = False" |
+"is_target ((s1,x,y,s2)#seq) q = (q = s2 \<or> is_target seq q)"
+
+definition visits :: "('in, 'out, 'state) FSM \<Rightarrow> 'state \<Rightarrow> ('state * 'in * 'out * 'state) list \<Rightarrow> 'state \<Rightarrow> bool" where
+"visits M s seq q \<equiv> is_enabled_sequence M s seq \<and> is_target seq q"
+
+definition reaches :: "('in, 'out, 'state) FSM \<Rightarrow> 'state \<Rightarrow> ('state * 'in * 'out * 'state) list \<Rightarrow> 'state \<Rightarrow> bool" where
+"reaches M s seq q \<equiv> is_enabled_sequence M s seq \<and> (case seq of
+  Nil \<Rightarrow> q = s |
+  _   \<Rightarrow> case (last seq) of (s1,x,y,s2) \<Rightarrow> q = s2)"
+
+
+
+
+
+
 definition well_formed :: "('in, 'out, 'state) FSM \<Rightarrow> bool" where
 "well_formed M \<equiv> 
     finite (states M)
@@ -18,6 +68,7 @@ definition well_formed :: "('in, 'out, 'state) FSM \<Rightarrow> bool" where
   (*\<and> (\<forall> (s1,x,y,s2) \<in> transitions M . 
       s1 \<in> states M \<and> s2 \<in> states M \<and> x \<in> inputs M \<and> y \<in> outputs M)*)
   \<and> transitions M \<subseteq> (states M) \<times> (inputs M) \<times> (outputs M) \<times> (states M)
+  \<and> (\<forall> s \<in> states M . \<exists> seq . reaches M (initial M) seq s)
 "
 
 lemma transition_finite : "well_formed M \<Longrightarrow> finite (transitions M)"
@@ -43,14 +94,12 @@ fun h_y :: "('in, 'out, 'state) FSM \<Rightarrow> 'state \<Rightarrow> 'in \<Rig
 
 
 definition observable :: "('in, 'out, 'state) FSM \<Rightarrow> bool" where
-(*"observable M \<equiv> \<forall> s1 \<in> states M . \<forall> x \<in> inputs M . \<forall> y \<in> outputs M . \<forall> s2a s2b . (s2a \<in> h_y M s1 x y \<and> s2b \<in> h_y M s1 x y) \<longrightarrow> s2a = s2b"*)
 "observable M \<equiv> \<forall> s1 x y s2 s3 . ((s1,x,y,s2) \<in> (transitions M) \<and> (s1,x,y,s3) \<in> (transitions M)) \<longrightarrow> s2 = s3"
 
 definition completely_specified :: "('in, 'out, 'state) FSM \<Rightarrow> bool" where
 "completely_specified M \<equiv> \<forall> s1 \<in> states M . \<forall> x \<in> inputs M . \<exists> y \<in> outputs M . \<exists> s2 \<in> states M . (s1,x,y,s2) \<in> transitions M"
 
 definition deterministic :: "('in, 'out, 'state) FSM \<Rightarrow> bool" where
-(*"deterministic M \<equiv> \<forall> s1 \<in> states M . \<forall> x \<in> inputs M . \<forall> ya s2a yb s2b . ((ya,s2a) \<in> h M s1 x \<and> (yb,s2b) \<in> h M s1 x) \<longrightarrow> (ya,s2a) = (yb,s2b)"*)
 "deterministic M \<equiv> \<forall> s1 x y1 y2 s2 s3 . ((s1,x,y1,s2) \<in> (transitions M) \<and> (s1,x,y2,s3) \<in> (transitions M)) \<longrightarrow> (s2 = s3 \<and> y1 = y2)"
 
 lemma observable_alt : "well_formed M \<Longrightarrow> observable M \<Longrightarrow> \<forall> s1 \<in> states M . \<forall> x \<in> inputs M . \<forall> y \<in> outputs M . (h_y M s1 x y = {}) \<or> (\<exists> s2 . h_y M s1 x y = {s2})"
@@ -58,43 +107,94 @@ lemma observable_alt : "well_formed M \<Longrightarrow> observable M \<Longright
   apply auto
   by (metis (mono_tags, lifting) Collect_cong singleton_conv)
 
+lemma get_io_length : "
+  well_formed M 
+  \<Longrightarrow> is_enabled_sequence M s seq 
+  \<Longrightarrow> io = get_io seq 
+  \<Longrightarrow> is_enabled_sequence M s seq2  
+  \<Longrightarrow> io = get_io seq2 
+  \<Longrightarrow> length seq = length seq2"
+  apply (simp)
+  by (metis length_map)
 
-inductive enabled_transition_seq :: "('in, 'out, 'state) FSM \<Rightarrow> 'state \<Rightarrow> (('in * 'out) * 'state) list => bool" where
-ets_nil  : "enabled_transition_seq M s Nil" |
-ets_one  : "(s1,x,y,s2) \<in> transitions M \<Longrightarrow> enabled_transition_seq M s1 (((x,y),s2)#Nil)" |
-ets_long : "(s1,x,y,s2) \<in> transitions M \<Longrightarrow> enabled_transition_seq M s2 seq \<Longrightarrow> enabled_transition_seq M s1 (((x,y),s2)#seq)"
+lemma observable_sequence1 : "
+  well_formed M 
+  \<Longrightarrow> observable M 
+  \<Longrightarrow> is_enabled_sequence M s ((s1,x11,y11,s2)#S1)
+  \<Longrightarrow> is_enabled_sequence M s ((t1,x12,y12,t2)#S2)  
+  \<Longrightarrow> get_io ((s1,x11,y11,s2)#S1) = get_io ((t1,x12,y12,t2)#S2)  
+  \<Longrightarrow> (s1,x11,y11,s2) = (t1,x12,y12,t2)"
+  by (auto simp: well_formed_def observable_def)
 
-inductive reachable :: "('in, 'out, 'state) FSM \<Rightarrow> 'state \<Rightarrow> bool" where
-reachable_init : "reachable M (initial M)" |
-reachable_immediately : "((initial M),x,y,s2) \<in> transitions M \<Longrightarrow> reachable M s2" |
-reachable_distant : "(s2,x,y,s3) \<in> transitions M \<Longrightarrow> reachable M s2 \<Longrightarrow> reachable M s3"
+lemma observable_sequence1c : "
+  well_formed M 
+  \<Longrightarrow> observable M 
+  \<Longrightarrow> is_enabled_sequence M s ((s1,x11,y11,s2)#S1)
+  \<Longrightarrow> is_enabled_sequence M s ((t1,x12,y12,t2)#S2)  
+  \<Longrightarrow> get_io ((s1,x11,y11,s2)#S1) = get_io ((t1,x12,y12,t2)#S2)  
+  \<Longrightarrow> S1 = S2
+  \<Longrightarrow> ((s1,x11,y11,s2)#S1) = ((t1,x12,y12,t2)#S2)"
+  by (auto simp: well_formed_def observable_def)
 
-inductive reaches :: "('in, 'out, 'state) FSM \<Rightarrow> ('in * 'out) list \<Rightarrow> 'state \<Rightarrow> bool" where
-reaches_nil : "reaches M Nil (initial M)" |
-reaches_transition : "reaches M seq s1 \<Longrightarrow> (s1,x,y,s2) \<in> transitions M \<Longrightarrow> reaches M (seq@((x,y)#Nil)) s2"
+lemma observable_sequence1d : "
+  well_formed M 
+  \<Longrightarrow> observable M 
+  \<Longrightarrow> is_enabled_sequence M s (a1#S1)
+  \<Longrightarrow> is_enabled_sequence M s (a2#S2)  
+  \<Longrightarrow> get_io (a1#S1) = get_io (a2#S2)  
+  \<Longrightarrow> S1 = S2
+  \<Longrightarrow> (a1#S1) = (a2#S2)"
+  apply (cases a1)
+  apply (cases a2)
+  by (auto simp: well_formed_def observable_def)
 
-lemma reachable_seq : "well_formed M \<Longrightarrow> reachable M s \<Longrightarrow> \<exists> seq . reaches M s seq" 
+lemma observable_sequence1e : "
+  well_formed M 
+  \<Longrightarrow> observable M 
+  \<Longrightarrow> is_enabled_sequence M s (a1#S1)
+  \<Longrightarrow> is_enabled_sequence M s S2  
+  \<Longrightarrow> get_io (a1#S1) = get_io S2  
+  \<Longrightarrow> S1 = tl S2
+  \<Longrightarrow> (a1#S1) = S2"
+  apply (cases a1)
+  by (auto simp: well_formed_def observable_def)
+
+
+lemma observable_sequence : "
+  well_formed M 
+  \<Longrightarrow> observable M 
+  \<Longrightarrow> is_enabled_sequence M s seq 
+  \<Longrightarrow> is_enabled_sequence M s seq2  
+  \<Longrightarrow> get_io seq = get_io seq2 
+  \<Longrightarrow> seq = seq2"
+proof (induction seq)
+  case Nil
+  then show ?case by auto
+next
+  case (Cons a seq)
+  
+  
+
+  (*then have "length (a # seq) = length seq2" by (meson get_io_length)*)
+  then show ?case sorry
+qed
+ 
+
+  apply (induction seq)
+   apply (simp)
+  apply (frule get_io_length)
+  apply auto
+
+  apply (frule observable_sequence1e)
+       apply auto
   apply sledgehammer
-  apply (induction rule: reachable.induct)
 
-definition reachable :: "('in, 'out, 'state) FSM \<Rightarrow> 'state \<Rightarrow> bool" where
-"reachable M s \<equiv> s = (initial M) \<or> (\<exists> seq . (enabled_transition_seq M (initial M) seq) \<and> s = snd (snd (last seq)))"
-
-
-
-fun apply_seq :: "('in, 'out, 'state) FSM \<Rightarrow> 'state \<Rightarrow> 'in list \<Rightarrow> ('in * 'out * 'state) list set" where
-"apply_seq M s1 Nil = {Nil}" |
-"apply_seq M s1 (x#xs) = {((x,y,s2)#res) | y s2 res . ((s1,x,y,s2) \<in> (transitions M) \<and> (res \<in> apply_seq M s2 xs))}"
-
-
-lemma apply_seq_input_const : "res \<in> apply_seq M s xs \<Longrightarrow> length xs = length res"
-  apply (induction xs)
-   apply auto
-  apply sledgehammer
-
-lemma apply_seq_input_const : "res \<in> apply_seq M s xs \<Longrightarrow> xs = map fst res"
-  apply (induction xs)
+  apply (cases seq2)
+   apply (simp add: well_formed_def observable_def)
   apply auto
   apply sledgehammer
+   apply (simp add: observable_def)
+  apply sledgehammer
+apply (auto simp: well_formed_def observable_def)
 
 end
